Eval array, set, object expressions
Signed-off-by: Anand Krishnamoorthi <anakrish@microsoft.com>

Rego.Interpreter.fst
@@ -5,3 +5,58 @@ module Rego.Interpreter
 
 open Rego.Ast
 open Rego.Value
+
+type intr=interpreter
+
+let make_new () = {
+   rules = [];
+   scopes = []
+}
+
+let rec eval_expr (e:expr) (i:intr)  : Tot (value*intr) =
+  match e with
+  | Var v -> lookup_var v i
+  | Value v -> (v, i)
+  | Ast.Array elems -> eval_array_elems elems [] i
+  | Ast.Set elems -> eval_set_elems elems [] i
+  | Ast.Object fields -> eval_fields fields (Object []) i
+  | _ -> (Undefined, i)
+
+and eval_array_elems (elems:list expr) (values:list value) (i:intr)  : Tot (value*intr)
+(decreases elems)
+=
+  match elems with
+  | [] -> (Value.Array (List.Tot.rev values), i)
+  | hd::tl -> 
+    match eval_expr hd i with
+    | (Undefined, i') -> (Undefined, i')
+    | (v, i') -> eval_array_elems tl (v::values) i'
+
+and eval_set_elems (elems:list expr) (values:list value) (i:intr)  : Tot (value*intr)
+(decreases elems)
+=
+  match elems with
+  | [] -> (List.Tot.fold_left Value.insert_into_set (Value.Set []) values, i)
+  | hd::tl -> 
+    match eval_expr hd i with
+    | (Undefined, i') -> (Undefined, i')
+    | (v, i') -> eval_set_elems tl (v::values) i'
+
+and eval_fields (fields:list (expr*expr)) (obj:value) (i:intr)  : Tot (value*intr)
+(decreases fields)
+=
+  match fields with
+  | [] -> (obj, i)
+  | (key_expr,value_expr)::tl -> 
+    match eval_expr key_expr i with
+    | (Undefined, i') -> (Undefined, i')
+    | (kv, i') -> 
+      match eval_expr value_expr i' with
+      | (Undefined, i'') -> (Undefined, i'')
+      | (vv, i'') -> eval_fields tl (insert_into_object obj kv vv) i''
+
+and lookup_var (ident:string) (i:intr)  : Tot (value*intr) (decreases ident) =
+  (Undefined, i)
+
+let eval (i:intr) (e:Ast.expr) : (value*intr) =
+  eval_expr e i
