Rego.Main.fst
@@ -13,6 +13,27 @@ let v2 = insert_at_path v1 (String "monde"::[]) v1
 let v3 = insert_at_path v2 (v2::[]) v2
 let v4 = Array (v1::v2::v3::[])
 
+let expr = Ast.Array (
+  Ast.Value (String "hello")::
+  Ast.Value (String "world")::
+  Ast.Array (
+    Ast.Value (Number 42)::
+    Ast.Set (
+      Ast.Value (Number 3)::
+      Ast.Value (Number 2)::
+      Ast.Value (Number 1)::
+      Ast.Object (
+        (Ast.Value (String "Hello"), Ast.Value (String "World"))
+        ::[]
+      )::
+      []      
+    )::[]
+  )::[]
+)
+
+let intr = Interpreter.make_new()
+let (v5, intr1) = Interpreter.eval intr expr
+
 let main () =
   FStar.IO.print_string (to_json_pretty v1);
   FStar.IO.print_string "\n";
@@ -21,6 +42,8 @@ let main () =
   FStar.IO.print_string (to_json_pretty v3);
   FStar.IO.print_string "\n";
   FStar.IO.print_string (to_json_pretty v4);
+  FStar.IO.print_string "\n";
+  FStar.IO.print_string (to_json_pretty v5);
   FStar.IO.print_string "\n"
   
 //Run ``main ()`` when the module loads
