Rego.Interpreter.fsti
@@ -1,0 +1,16 @@
+// Copyright (c) Microsoft Corporation.
+// Licensed under the MIT License.
+
+module Rego.Interpreter
+
+type scope = FStar.Map.t string Value.value
+
+noeq
+type interpreter = {
+  rules: list (string*Ast.rule);
+  scopes: list scope;
+}
+
+val make_new () : interpreter
+
+val eval (i:interpreter) (e:Ast.expr) : (Value.value*interpreter)
