build_and_run.sh
@@ -2,8 +2,10 @@
 
 set -e
 
-fstar.exe  --codegen OCaml --extract "Rego"  --odir out Rego.Value.fst 
+fstar.exe  --codegen OCaml --extract "Rego"  --odir out Rego.Value.fst
 fstar.exe  --codegen OCaml --extract "Rego"  --odir out Rego.Main.fst
+fstar.exe  --codegen OCaml --extract "Rego"  --odir out Rego.Ast.fst
+fstar.exe  --codegen OCaml --extract "Rego"  --odir out Rego.Interpreter.fst
 
 cd out
 export OCAMLPATH="dirname $(which fstar.exe)"
